\documentclass{article}
\usepackage{graphicx}
\usepackage{amsmath}
\usepackage{amsfonts}
\usepackage{bm}
\usepackage[margin=1in]{geometry}
\usepackage{parskip}
\usepackage{algorithm}
\usepackage{algpseudocode}

\usepackage[backend=biber,style=numeric,sorting=ynt,bibencoding=utf8]{biblatex}
\addbibresource{sources.bib}

\renewcommand\aa{\bm{\theta}}
\renewcommand\t{\vartheta}
\newcommand\R{\bm{R}}
\newcommand\q{\bm{q}}
\newcommand\I{\bm{I}}
\renewcommand\u{\bm{u}}
\renewcommand\v{\bm{v}}
\renewcommand\skew[1]{[#1]_{\times}}
\newcommand\Real{\mathbb{R}}
\newcommand\norm[1]{\Vert#1\Vert}
\newcommand\vecop[1]{\text{vec} \left( #1\right)}

\DeclareMathOperator{\arctantwo}{arctan2}

\begin{document}

\title{Overview of 3D orientation transformations with Jacobians}
\author{Christian V. Berg}
\maketitle
\date

Many of the following transformations are functions of matricies. Since we are
also interested in their first order derivative, we need an efficient way
of ordering their partial derivates. In the following derivations, we use the
\textit{Magnus-Neudecker} layout convention as presented in
\cite{magnus_matrix_1985}. A practical introduction can be found in
\cite{fackler_notes_2005}. We will be using the product rule in particular: Given 
functions $f(X):\Real^{n \times m} \to \Real^{p \times q}$ and
$g(X):\Real^{n \times m} \to \Real^{q \times k}$ then
\begin{align}
  \frac{\partial \vecop{f(X) g(X)}}{\partial \vecop{X}} =
    \left(g(X)^T \otimes \bm{I}_k \right) \frac{\partial \vecop{f(X)}}{\partial \vecop{X}}
    + \left(\bm{I}_p \otimes f(X) \right) \frac{\partial \vecop{g(X)}}{\partial \vecop{X}}
\end{align}

where $\otimes$ is the Kronecker product. You will also find some references to the Lie group $SO(3)$ and its exponential map.
Though Lie theory is not needed to understand what follows, an excellent introduction
to the topic and its applications in robotics can be found in \cite{sola_micro_2019}.


\tableofcontents

\section{Notations}
\subsection{Symbols}
\begin{tabular}{l p{15cm}}
  $\t \in \Real$ & Angle \\
  $\aa \in \Real^3$ & Axis-angle such that $\aa = \t \, \u$, $\t \in \Real$ and a unit vector $\u \in S^2$ \\
  $\q \in S^3$ & Unit quaternion such that $\q = \begin{bmatrix} w \\ \v \end{bmatrix}$ \\
  $\R \in SO(3)$ & Rotation matrix \\
  $\I \in \Real^{3\times3}$ & Identity matrix \\
  $\bm{0} \in \Real^{3}$ & Zero vector \\
  $\bm{1} \in \Real^{3}$ & Vector of ones \\
   $e_i \in \Real^3$ & $i^{th}$ standard orthonormal base vector of $\Real^3$, i.e.
     $e_1=\begin{bmatrix} 1 \\ 0 \\ 0 \end{bmatrix},
     e_2 =\begin{bmatrix} 0 \\ 1 \\ 0 \end{bmatrix},
       e_3 =\begin{bmatrix} 0 \\ 0 \\ 1 \end{bmatrix}$ \\ [10pt] \\
   $E_i = \skew{e_i}\in \Real^{3 \times 3}$ & $i^{th}$ generator of $SO(3)$ \\ [10pt] \\
\end{tabular}

\subsection{Operators}
\begin{tabular}{l p{15cm}}
  $ (.)^T : \Real^{m \times n} \to \Real^{n \times m}$ & Matrix transpose \\
  $tr(.) : \Real^{n \times n} \to \Real$ & Matrix trace \\
  $\skew{.} : \Real^3 \to  \Real^{3\times 3}$ & Skew symmetric matrix operator such that
  $\begin{bmatrix} x \\ y \\ z \end{bmatrix}_\times =
  \begin{bmatrix}
    0& - z & y \\ 
    z & 0 & -x \\
    -y & x & 0
  \end{bmatrix}$ \\ [10pt] \\
  $(.)^\vee : \Real^{3 \times 3} \to \Real^{3}$ & Vee operator such that
  $\begin{bmatrix}
    a_1& - z & y \\ 
    z & a_2 & -x \\
    -y & x & a_3
  \end{bmatrix}^\vee = \begin{bmatrix} x \\ y \\ z \end{bmatrix}$ \newline Notice that $\left(\skew{\bm{d}}\right)^\vee = \bm{d}$ \\
    $\vecop{.} : \Real^{m \times n} \to \Real^{m\,n}$ & Vectorization operator of a matrix such that
   $\vecop{\begin{bmatrix}
    a_1 & a_3 \\ 
    a_2 & a_4
    \end{bmatrix}} = \begin{bmatrix} a_1 \\ a_2 \\ a_3 \\ a_4 \end{bmatrix}$ \\ [10pt] \\
\end{tabular}

\section{Rotation matrix and axis-angle}
\subsection{Rotation matrix from axis-angle}
This transformation is provided by Rodrigues' rotation formula, and gives a closed form expression of the exponential map of $SO(3)$:
\begin{align}
  \R = \exp(\skew{\aa}) = \I + \frac{\sin \t}{\t} \skew{\aa} + \frac{1 - \cos \t}{\t^2} \skew{\aa}^2 
\end{align}

First order Taylor approximation at $\aa = \bm{0}$
\begin{align}
  \R = \exp(\skew{\aa}) = \I + \skew{\aa} + O(\skew{\aa}^2) \approx \I + \skew{\aa}
\end{align}

\subsection{Rotation matrix from axis-angle Jacobian}
Since the expression is fairly long, we will define 2 intermediate functions:
\begin{align}
  k_1(\t) = \frac{\sin{\t}}{\t} \;\;&,\;\;
  \frac{\partial k_1(\t)}{\partial \t} = \frac{\t\cos{\t} - \sin{\t}}{\t^2} \\
  k_2(\t) = \frac{1-\cos{\t}}{\t^2} \;\;&,\;\;
  \frac{\partial k_2(\t)}{\partial \t} = \frac{\t\sin{\t} - 2\left(1-\cos{\t} \right)}{\t^3}
\end{align}

For both functions, we have
\begin{align}
  \frac{\partial k_i(\t)}{\partial \aa} &= 
    \frac{\partial k_i(\t)}{\partial \t} \frac{\t}{\partial \aa} =
    \frac{\partial k_i(\t)}{\partial \t} \frac{\sqrt{\aa^T\aa}}{\partial \aa} =
    \frac{\partial k_i(\t)}{\partial \t} \frac{\aa^T}{\t}
\end{align}

Using the Kronecker product $\otimes$, it then follows
\begin{align}
  \frac{\partial \vecop{k_1(\t) \skew{\aa}}}{\partial \aa}  
  &= \left( \I \otimes k_1(\t)\I \right) \frac{\partial \vecop{\skew{\aa}}}{\partial \aa}
    + \left(\skew{\aa}^T \otimes \I \right) \frac{\partial \vecop{k_1(\t)\;\I}}{\partial \aa} \\
  &= k_1(\t) \frac{\partial \vecop{\skew{\aa}}}{\partial \aa}
    - \left(\skew{\aa} \otimes \I \right) \vecop{\I} \frac{\partial k_1(\t)}{\partial \t} \frac{\aa^T}{\t}
\end{align}

where we used $\skew{.}^T = - \skew{.}$. Next, we also have
\begin{align}
  \frac{\partial \vecop{k_2(\t) \skew{\aa}^2}}{\partial \aa}  
  &= \left( \I \otimes k_2(\t)\I \right) \frac{\partial \vecop{\skew{\aa}^2}}{\partial \aa}
    + \left({\skew{\aa}^2}^T \otimes \I \right) \frac{\partial \vecop{k_2(\t)\;\I}}{\partial \aa} \\
  &= k_2(\t) \frac{\partial \vecop{\skew{\aa}^2}}{\partial \aa}
    + \left({\skew{\aa}^2} \otimes \I \right) \vecop{\I} \frac{\partial k_2(\t)}{\partial \t} \frac{\aa^T}{\t}
\end{align}

where we used ${\skew{.}^2}^T = \skew{.}^2$. Putting it all together, we get:

\begin{align}
  \frac{\partial \vecop{\R}}{\partial \aa} = 
    \frac{\partial \vecop{k_1(\t) \skew{\aa}}}{\partial \aa}  
    + \frac{\partial \vecop{k_2(\t) \skew{\aa}^2}}{\partial \aa}  
\end{align}

When $\t = 0$, we reuse the exponential map of $SO(3)$ to deduce that 
\begin{align}
  \left. \frac{\partial \vecop{\R}}{\partial \aa} \right \vert_{\aa = \bm{0}} =
  \left. \frac{\partial \vecop{\exp(\skew{\aa})}}{\partial \aa_i} \right \vert_{\aa = \bm{0}} \approx
  \left. \frac{\partial \vecop{\I + \skew{\aa}}}{\partial \aa_i} \right \vert_{\aa = \bm{0}} =
  \frac{\partial \vecop{\skew{\aa}}}{\partial \aa}
\end{align}

\subsection{Axis-angle from rotation matrix}
We begin by retrieving the angle $\t$:
\begin{align}
  tr(\R) 
    &= tr(\I) + \frac{\sin \t }{\t} tr(\skew{\aa}) + \frac{1 - \cos \t}{\t^2} tr(\skew{\aa}^2) \\
    &= 3 - 2 (1 - \cos \t) \\
  \t &=  \arccos \frac{tr(\R) - 1}{2}
\end{align}

where we used $tr(\skew{\aa}^2) =  - 2 \aa^T \aa = -2\t^2$ and $tr(\skew{.}) = 0$.

Next, and assuming $\t \neq 0 \iff tr(\R) \neq 3$ and $\t \neq \pi \iff tr(\R) \neq -1$ then
\begin{align}
  \R - \R^T 
    &= \frac{\sin{\t}}{\t} \left(\skew{\aa} - \skew{\aa}^T\right)
    + \frac{1 - \cos \t}{\t^2} \left( \skew{\aa}^2 - \skew{\aa}^{2^T} \right) \\
    &= \frac{2\, \sin \t}{\t} \skew{\aa} \\
  \aa &= \frac{\t \, \left(\R - \R^T \right)^\vee }{2\, \sin \t}
\end{align}

When $\t$ is close to $0 \iff tr(\R)$ close to $3$, we can reuse the first
order Taylor approximation from before:

\begin{align}
  \aa \approx \left( \R - \I \right)^\vee
\end{align}

When $\t = \pi \iff tr(\R) = -1$
\begin{align}
  \R = \I + \frac{2}{\t^2} \skew{\aa}^2 
  &= \I + 2\skew{\u}^2 \\
  &= \I + 2\, (\u \u^T - \I) \\
  \u \u^T = \frac{\R + \I }{2}
\end{align}

where we used $\skew{\u}^2 =  \u \u^T - \u^T \u \I$ and $\u^T \u = 1$ by definition.
Since $\u \u^T$ has the form:
\begin{align}
  \u \u^T = 
  \begin{bmatrix}
    \u_x^2 & \u_x \u_y & \u_x \u_z \\
    \u_y \u_x & \u_y^2 & \u_y \u_z \\
    \u_z \u_x & \u_z \u_y & \u_z^2
  \end{bmatrix}
\end{align}

we know that the largest element of the diagonal corresponds to the most
significant axis of rotation. Since $\t=\pi$ then the largest diagonal element
is always different from zero. Therefore, we take the square root of the largest
diagonal element, then use it to divide its corresponding column vector in
order to retrieve $\u$. Note that we cannot deduce the sign of $\u$, only the
relative "sign-ness" of each element.

\begin{align}
  \u = \pm 
    \frac{col_i \left[ \frac{\R + \I}{2} \right] }
         {\sqrt{diag_i \left[ \frac{\R + \I }{2} \right] }}
  \;,\; i = argmax \;\; diag \left( \frac{\R + \I }{2} \right)
\end{align}

Finally
\begin{align}
  \aa = \pm \pi \u
\end{align}

\subsection{Axis-angle from rotation matrix Jacobian}
Once again we will define an intermediate function and variable:
\begin{align}
  k_3(\t) = \frac{\t}{2\sin{\t}} \;\;&,\;\;
  \frac{\partial k_3(\t)}{\partial \t} = 
    \left(1 - \frac{\t}{\tan{\t}} \right) \frac{1}{2\sin{\t}} \\
  x = \frac{tr(\R) - 1}{2} \;\;&,\;\; \t = \arccos(x)
\end{align}

Consequently, we have
\begin{align}
  \frac{\partial k_3(\t)}{\partial tr(\R)} 
  &=\frac{\partial k_3(\t)}{\partial \t} 
    \frac{\partial \t}{\partial x} 
    \frac{\partial x}{\partial tr(\R)} \\
  &=-\frac{\partial k_3(\t)}{\partial \t} 
    \frac{1}{2\sqrt{1-\t^2}}
\end{align}

Assuming $\t \neq 0 \iff tr(\R) \neq 3$ and $\t \neq \pi \iff tr(\R) \neq -1$, then
\begin{align}
  \frac{\partial \vecop{\aa}}{\partial \vecop{\R}} = 
    \big({(\R - \R^T)^\vee}^T \otimes \I \big)
    \vecop{\I}
    \frac{\partial k_3(\t)}{\partial tr(\R)} 
    \frac{\partial tr(\R)}{\partial \vecop{\R}} + 
    k_3(\t) \frac{\partial \left( \R - \R^T \right)^\vee}{\partial \vecop{\R}}
\end{align}

When $\t = 0 \iff tr(\R) = 3$, then 
\begin{align}
  \left. \frac{\partial \aa}{\partial \vecop{\R}} \right \vert_{\aa = \bm{0}} \approx
    \frac{\partial \left(\R - \I \right)^\vee}{\partial \vecop{\R}}
\end{align}

\section{Rotation matrix and quaternion}
\subsection{Rotation matrix from quaternion}
Assuming unit quaternions, we have
\begin{align}
  \R = \I + 2 \; w \; \skew{\v} + 2\; \skew{\v}^2
\end{align}

\subsection{Rotation matrix from quaternion Jacobian}
\begin{align}
  \frac{\partial \vecop{\R}}{\partial w} &= 2\, \vecop{\skew{\v}} \\
  \frac{\partial \vecop{\R}}{\partial \v} &= 
  2w \frac{\partial\vecop{\skew{\v}}}{\partial \v} +
  2 \frac{\partial\vecop{\skew{\v}^2}}{\partial \v} \\
  \frac{\partial \vecop{\R}}{\partial \q} &= 
    \begin{bmatrix}
      \frac{\partial \vecop{\R}}{\partial w} & 
      \frac{\partial \vecop{\R}}{\partial \v}
    \end{bmatrix}
\end{align}

\subsection{Quaternion from rotation matrix}
We begin by retrieving the scale component of the quaternion:
\begin{align}
  tr(\R) 
    &= tr(\I) + 2\; w \; tr(\skew{\v}) + 2 \; tr(\skew{\v}^2) \\
    &= 3 - 4 \v^t \v = 4\;w^2 - 1 \\
  w &= \pm \frac{ \sqrt{ tr(\R) + 1} }{2}
\end{align}

Assuming $w \neq 0 \iff tr(\R) \neq -1$
\begin{align}
  \R - \R^T
    &= 2\; w \; \left( \skew{\v} - \skew{\v}^T \right) + 2 \; \left(\skew{\v}^2 - {\skew{\v}^2}^T \right) \\
    &= 4\; w \; \skew{\v} \\
  \v &= \frac{\left( \R -\R^T \right)^\vee}{4\;w}
\end{align}

When $w = 0$, then
\begin{align}
  \R &= \I + 2 \skew{\v}^2  = \I + 2 \left ( \v \v^T - \I \right) \\
  \v \v^T &= \frac{\R + \I}{2}
\end{align}

and we can reuse the same method as for axis-angle when $\t = \pi$.

\subsection{Quaternion from rotation matrix Jacobian}
As before, we define
\begin{align}
  k_4(w) = \frac{1}{4w} \;\;,\;\; \frac{\partial k_4(w)}{\partial w} = -\frac{1}{4w^2}
\end{align}

Assuming $w \neq 0 \iff tr(\R) \neq -1$
\begin{align}
  \frac{\partial w}{\partial \vecop{\R}}
    &=\frac{\partial w}{\partial tr(\R)} \frac{\partial tr(\R)}{\partial \vecop{\R}}
    = \frac{1}{4\sqrt{tr(\R) + 1}} \frac{\partial tr(\R)}{\partial \R} \\
  \frac{\partial \v}{\partial \vecop{\R}}
    &= \big({\left(\R - \R^T\right)^\vee}^T \otimes \I \big)\frac{\partial k_4(w)}{\partial w}\frac{\partial w}{\partial \vecop{\R}}
    + k_4(w) \frac{\partial \left(\R - \R^T\right)^\vee }{\partial \vecop{\R}}
\end{align}

\section{Axis-angle and quaternion}
\subsection{Quaternion from axis-angle}
\begin{align}
  \q = 
    \begin{bmatrix} 
       \cos{ \frac{\t}{2} } \\[5pt]
       \frac{\sin{ \frac{\t}{2} }}{\t} \aa
    \end{bmatrix}
\end{align}

When $\t$ is close to $0$, then the second order Taylor approximation is
\begin{align}
  \q \approx
    \begin{bmatrix} 
      1 - \frac{\t^2}{8} \\[5pt]
      \left( \frac{1}{2} - \frac{\t^2}{48} \right) \aa
    \end{bmatrix}
\end{align}

\subsection{Quaternion from axis-angle Jacobian}
\begin{align}
  \frac{\partial w}{\partial \aa} 
  &=  \frac{\partial w}{\partial \t} \frac{\partial \t}{\partial \aa}  \\
  &=-\frac{\sin{\frac{\t}{2}}}{2} \frac{\aa^T}{\t}  \\
     \frac{\partial \v}{\partial \aa} &= 
  \aa \frac{\partial \frac{\sin{ \frac{\t}{2} }}{\t}}{\partial \aa} + 
  \frac{\sin{ \frac{\t}{2} }}{\t} \frac{\partial \aa}{\partial \aa}\\
  &= \aa \frac{\partial \frac{\sin{ \frac{\t}{2} }}{\t}}{\partial \t} \frac{\partial \t}{\partial \aa}  + 
  \frac{\sin{ \frac{\t}{2} }}{\t} \I \\
  &= 
     \aa \frac{\t \, \cos{\frac{\t}{2}} - 2\,\sin{\frac{\t}{2}}}{2\,\t^2} \frac{\aa^T}{\t}
    + \frac{\sin{\frac{\t}{2}}}{\t} \I
\end{align}

When $\t$ is close to $0$, then
\begin{align}
  \left. \frac{\partial w}{\partial \aa} \right \vert_{\aa = 0} &\approx - \frac{1}{4} \aa^T \\
  \left. \frac{\partial w}{\partial \aa} \right \vert_{\aa = 0} &\approx - \frac{1}{24} \aa \aa^T + \left(\frac{1}{2} - \frac{\t^2}{48} \right) \I
\end{align}

and finally

\begin{align}
  \frac{\partial \q}{\partial \aa} = 
    \begin{bmatrix}
      \frac{\partial w}{\partial \aa} \\[5pt]
      \frac{\partial \v}{\partial \aa}
    \end{bmatrix}
\end{align}

\subsection{Axis-angle from quaternion}
Using $y=\sqrt{\v^T\v}$
\begin{align}
  \aa = 2 \frac{\arctantwo \left(y, w \right)}{y} \v 
\end{align}

When $w$ approaches $1$ from the left $\iff \t$ close to $0$, we can reuse the second order Taylor approximation from before to deduce
\begin{align}
  \aa \approx \frac{6\v}{w+2}
\end{align}

\subsection{Axis-angle from quaternion Jacobian}
We define an intermediate function
\begin{align}
  k_5(y,x) &= 2 \frac{\arctantwo \left(y, w \right)}{y} \\
  \frac{\partial k_5(y,x)}{\partial x} &= \frac{-2}{y^2 + w^2} = -2 \\
  \frac{\partial k_5(y,x)}{\partial y} &= 2 \frac{ \frac{w\,y}{y^2 + w^2} - \arctantwo \left(y, w \right)}{y^2} = 2 \frac{ w\,y - \arctantwo \left(y, w \right)}{y^2}
\end{align}
where we used $y^2 + w^2 = \q^T \q = 1$ since we are assuming unit quaternions. It then follows:
\begin{align}
  \frac{\partial \aa}{\partial w} &= \frac{\partial k_5(y,w)}{\partial w} \v \\
  \frac{\partial \aa}{\partial \v} 
  &= \v \frac{\partial k_5(y,w)}{\partial y} \frac{\partial y}{\partial \v} + k_5(y,w) \I
  =  \v \frac{\partial k_5(y,w)}{\partial y} \frac{\v^T}{y} + k_5(y,w) \I
\end{align}

When $w$ approach $1$ from the left $\iff \t$ close to $0$, then
\begin{align}
  \left. \frac{\partial \aa}{\partial w} \right \vert_{w = 1^-} &\approx - \frac{6}{\left( w + 2 \right)^2} \v \\
  \left. \frac{\partial \aa}{\partial \v} \right \vert_{w = 1^-} &\approx \frac{6}{w + 2} \I
\end{align}

and finally

\begin{align}
  \frac{\partial \aa}{\partial \q} = 
    \begin{bmatrix}
      \frac{\partial \aa}{\partial w} &
      \frac{\partial \aa}{\partial \v}
    \end{bmatrix}
\end{align}

\section{Euler angles and rotation matrix}

This section is largely based on \cite{eberly_euler_nodate}, which details how
one can retrieve the euler angles of a given sequence of rotation from a rotation matrix.

The following subsection presents the psudocode to retrieve the wanted euler angles, but 
unlike \cite{eberly_euler_nodate}, the psudocode is generalized for the order of rotation.

We define

\begin{tabular}{l p{15cm}}
  $\R_i(\t_k)$ & The rotation matrix about the axis $e_i$ by an angle $\t_k$ \\
  $s_k$ & Sine of the angle $\t_k$, i.e. $s_k = \sin \t_k$\\
  $c_k$ & Cosine of the angle $\t_k$, i.e. $c_k = \cos \t_k$\\
  $M$ & The "sign" matrix used to correct the sign of the sine and cosine element of the rotation matrix \\
\end{tabular}

Using this, a rotation matrix can be written as $\R = \R_a(\t_1) \; \R_b(\t_2) \; \R_c(\t_3)$.
For example, the sequences of rotation \textit{z-y-x} by angles $(\t_3, \t_2, \t_1)$ is written
$\R = \R_1(\t_1) \; \R_2(\t_2) \; \R_3(\t_3)$.


A particular matrix element is denoted by a lower case letter and the indicies in subscript, i.e.
\begin{align}
  \R = \begin{bmatrix} 
    r_{1,1} & r_{1,2} & r_{1,3} \\
    r_{2,1} & r_{2,2} & r_{2,3} \\
    r_{3,1} & r_{3,2} & r_{3,3}
  \end{bmatrix} \text{       }
\end{align}

The both algorithms rely on a sign matrix given by
\begin{align}
  M = \begin{bmatrix} 
    m_{1,1} & m_{1,2} & m_{1,3} \\
    m_{2,1} & m_{2,2} & m_{2,3} \\
    m_{3,1} & m_{3,2} & m_{3,3}
  \end{bmatrix} 
  = \begin{bmatrix} 
    1 & -1 & 1 \\
    1 & 1 & -1 \\
    -1 & 1 & 1
  \end{bmatrix} = 
  \I + \skew{\bm{1}}
\end{align}

\subsection{Tait-Bryan angles from rotation matrix}

\begin{algorithm}[H]
\begin{algorithmic}[1]
\Function{ToTaitBryan}{$\R,a,b,c$}\Comment{Corresponds to the rotation sequence $e_c-e_b-e_a$}
  \State $M = \I + \skew{\bm{1}}$\Comment{Sign matrix}
  \State $s_2 = r_{a,c}$
  \If{$s_2 < +1$}
    \If{$s_2 > -1$}
      \State $\t_2 = \arcsin(m_{a,c} \; s2)$
      \State $\t_1 = \arctantwo(m_{b,c} \; r_{b,c}, m_{c,c} \; r_{c,c})$
      \State $\t_3 = \arctantwo(m_{a,b} \; r_{a,b}, m_{a,a} \; r_{a,a})$
    \Else\Comment{Gimbal lock: $s_2 = -1$}
      \State $\t_2 = - m_{a,c} \; \frac{\pi}{2}$
      \State $\t_1 = \arctantwo(m_{b,a} \; r_{b,a}, m_{b,b} \; r_{b,b})$
      \State $\t_3 = 0$
    \EndIf
  \Else\Comment{Gimbal lock: $s_2 = 1$}
    \State $\t_2 = m_{a,c} \; \frac{\pi}{2}$
    \State $\t_1 = \arctantwo(m_{b,a} \; r_{b,a}, m_{b,b} \; r_{b,b})$
    \State $\t_3 = 0$
  \EndIf
  \State \textbf{return} $\t_1, \t_2, \t_3$
\EndFunction
\end{algorithmic}
\end{algorithm}

\subsection{Proper Euler angles from rotation matrix}

\begin{algorithm}[H]
\begin{algorithmic}[1]
  \Function{ToProperEuler}{$\R,a,b$}\Comment{Corresponds to the rotation sequence $e_a-e_b-e_a'$}
  \State $M = \I + \skew{\bm{1}}$\Comment{Sign matrix}
  \State $c = 6 - a -b$\Comment{$c$ is the "unused" axis}
  \State $c_2 = r_{a,a}$
  \If{$c_2 < +1$}
    \If{$c_2 > -1$}
      \State $\t_2 = \arccos(m_{a,a} \; c2)$
      \State $\t_1 = \arctantwo(m_{b,a} \; r_{b,a}, m_{c,a} \; r_{c,a})$
      \State $\t_3 = \arctantwo(m_{a,b} \; r_{a,b}, m_{a,c} \; r_{a,c})$
    \Else\Comment{Gimbal lock: $c_2 = -1$}
      \State $\t_2 = \pi$
      \State $\t_1 = - \arctantwo(m_{b,c} \; r_{b,c}, m_{b,b} \; r_{b,b})$
      \State $\t_3 = 0$
    \EndIf
  \Else\Comment{Gimbal lock: $c_2 = 1$}
    \State $\t_2 = 0$
    \State $\t_1 = \arctantwo(m_{b,c} \; r_{b,c}, m_{b,b} \; r_{b,b})$
    \State $\t_3 = 0$
  \EndIf
  \State \textbf{return} $\t_1, \t_2, \t_3$
\EndFunction
\end{algorithmic}
\end{algorithm}

\newpage

\section{Common matrix derivatives}

Using $e'_i$ as $i^{th}$ standard orthonormal base vector of $\Real^9$, then

\begin{align}
  \forall X \in \Real^{3 \times 3} \;\; \text{ then } \;\; \frac{\partial \vecop{X^T}}{\partial \vecop{X}}
  = \begin{bmatrix} e'_1 &   e'_4 &   e'_7 &   e'_2 &   e'_5 &   e'_8 &   e'_3 &   e'_6 &   e'_9  \end{bmatrix} = J_T
\end{align}

\begin{align}
  \forall X \in \Real^{n \times n} \;\; \text{ then } \;\; \frac{\partial \vecop{tr(X)}}{\partial \vecop{X}}
  = \vecop{\I_n}
\end{align}

\begin{align}
  \forall \bm{v} \in \Real^{3} \;\; \text{ then } \;\; \frac{\partial \skew{\bm{v}}}{\partial \bm{v}}
  = \begin{bmatrix} \vecop{E_1} &  \vecop{E_2} & \vecop{E_3} \end{bmatrix} = J_\times
\end{align}

\begin{align}
  \forall X \in \Real^{3 \times 3} \;\; \text{ then } \;\; \frac{\partial X^\vee}{\partial \vecop{X}} =
  \begin{bmatrix}
    0 & 0 & 0 & 0 & 0 & 0 & 0 & -1 & 0 \\
    0 & 0 & 0 & 0 & 0 & 0 & 1 & 0 & 0 \\
    0 & 0 & 0 & 0 & -1 & 0 & 0 & 0 & 0
  \end{bmatrix} = J_\vee
\end{align}

\begin{align}
  \forall X \in \Real^{3 \times 3} \;\; \text{ then } \;\; \frac{\partial (X - X^T)^\vee}{\partial \vecop{X}}
  = \frac{\partial (X - X^T)^\vee}{\partial \vecop{X - X^T}}
  \frac{\partial \vecop{X - X^T}}{\partial \vecop{X}} = J_\vee \; (\I_9 - J_T)
\end{align}


\printbibliography

\end{document}
